comm

HeapInsert.dfy
@@ -2,6 +2,7 @@
 
 method {:verify true} Parent(index: nat) returns (p: int) 
 	ensures p == (index - 1) / 2
+	ensures p <= index
 {
 	p := (index - 1) / 2;
 }
@@ -23,181 +24,204 @@ predicate hp(q: seq<int>, length: nat)
 predicate ph(q: seq<int>, s: set<nat>)
 	requires (forall e :: e in s ==> e < |q|)
 {
-	forall i,j :: i in s && j in s && AncestorIndex(i, j) ==> q[i] >= q[j]
+	(forall i,j :: i in s && j in s && AncestorIndex(i, j) ==> q[i] >= q[j])
+}
+
+predicate phAndHi(q: seq<int>, s: set<nat>, k: nat)
+	requires (forall e :: e in s ==> e < |q|)
+{
+	(forall i,j :: i in s && j in s && AncestorIndex(i, j) ==> q[i] >= q[j]) &&
+	forall j :: j in s && AncestorIndex(k, j) ==> q[k] >= q[j]
 }
 // element k is a valid heap element (in the given range) with respect to its ancestors (lower indices)
-predicate lo(q: seq<int>, l: nat, h: nat, k: nat)
-	requires l <= h <= |q| && k < |q|
+predicate lo(q: seq<int>, s: set<nat>, k: nat)
+    requires k < |q| && (forall e :: e in s ==> e < |q|)
 {
-	forall i :: l <= i < h && AncestorIndex(i, k) ==> q[i] >= q[k]
+	forall i :: i in s && AncestorIndex(i, k) ==> q[i] >= q[k]
 }
 // element k is a valid heap element (in the given range) with respect to its descendents (higher indices)
-predicate hi(q: seq<int>, l: nat, h: nat, k: nat)
-	requires l <= h <= |q| && k < |q|
+predicate hi(q: seq<int>, s: set<nat>, k: nat)
+	requires k < |q| && (forall e :: e in s ==> e < |q|)
 {
-	forall j :: l <= j < h && AncestorIndex(k, j) ==> q[k] >= q[j]
+	forall j :: j in s && AncestorIndex(k, j) ==> q[k] >= q[j]
 }
 // the suffix q[i..] holds elements in their final (sorted) positions
-//fn
+
 function IndexSet(start: nat, end: nat, except: nat): set<nat> {
 	 set i: nat | start <= i < end && i != except }
 
-method {:verify false} swap (a: array<int>, heapsize: nat, x: int, current: nat, parentIndex: int, oldA: seq<int>) 
-	requires 0 <= current < a.Length && 0 < heapsize <= a.Length && 0 <= parentIndex < a.Length
-	requires Guard1(a,current,parentIndex) && WhileInv(a[..],heapsize,x,current,parentIndex,oldA)
-	ensures current > 0 && WhileInv(a[..],heapsize,x,current,parentIndex,oldA)
-	modifies a
-{
-	Lemma3(a,heapsize,x,current,parentIndex,oldA);
-	a[current], a[parentIndex] := a[parentIndex], a[current];
-}
-
-method {:verify true} HeapInsert(a: array<int>, heapsize: nat, x: int)
-	requires 0 <= heapsize < a.Length
+method HeapInsert(a: array<int>, heapsize: nat, x: int)
+	requires heapsize < a.Length
 	requires hp(a[..], heapsize)
 	ensures hp(a[..], heapsize+1)
 	ensures multiset(a[..heapsize+1]) == multiset(old(a[..heapsize])+[x])
 	modifies a
 {
-	// BottomInsertLemma(a ,heapsize, x);
-	var newHeapsize := BottomInsert(a, heapsize, x);
-	HeapInsert1(a, newHeapsize, x);	
+    // Sequantial Composition
+    HeapInsert1a(a, heapsize, x);	
+	HeapInsert1b(a, heapsize + 1, x, multiset(old(a[..heapsize])+ [x]));	
 }
-method {:verify true} BottomInsert(a: array<int>, heapsize0: nat, x: int) returns (heapsize: nat)
-	requires 0 <= heapsize0 < a.Length
-	requires hp(a[..], heapsize0)
-	ensures heapsize0 < heapsize && heapsize <= a.Length
-	ensures multiset(a[..heapsize]) == multiset(old(a[..heapsize - 1])+[x])
-	ensures a[heapsize-1] == x && 0 < heapsize <= a.Length
-	ensures hp(a[..], heapsize-1) && ph(a[..heapsize], IndexSet(0, heapsize, heapsize-1))
-	modifies a
+
+method HeapInsert1a(a: array<int>, heapsize: nat, x: int)
+    requires heapsize < a.Length
+	requires hp(a[..], heapsize)
+    ensures 0 < heapsize + 1 <= a.Length
+    ensures multiset(a[..heapsize+1]) == multiset(old(a[..heapsize])+[x])
+    ensures phAndHi(a[..heapsize+1], IndexSet(0, heapsize+1, heapsize), heapsize)
+    modifies a
 {
-	// Lemma1(a, heapsize0+1, x);
-	a[heapsize0] := x;
-	heapsize := heapsize0 + 1;
+    // Assignment
+    Lemma1(a, heapsize, x);
+    a[heapsize] := x;
 }
 
-// lemma Lemma1 (a: array<int>, heapsize: nat, x: int)
-// 	requires 0 <= heapsize - 1  < a.Length
-// 	requires hp(a[..], heapsize - 1)
+lemma Lemma1 (a: array<int>, heapsize: nat, x: int)
+    requires heapsize < a.Length
+	requires hp(a[..], heapsize)
+    ensures var newA := a[..heapsize]+[x]; 0 < heapsize + 1 <= |newA| && 
+    multiset(newA) == multiset(a[..heapsize]+[x]) && 
+    phAndHi(newA[..heapsize+1], IndexSet(0, heapsize+1, heapsize), heapsize)
+{}
 
-// {}
-
-method {:verify true} HeapInsert1(a: array<int>, heapsize: nat, x: int)
-	requires 0 < heapsize <= a.Length && a[heapsize-1] == x
-	requires multiset(a[..heapsize]) == multiset(a[..heapsize-1]+[x])
-	requires hp(a[..], heapsize-1) && ph(a[..heapsize], IndexSet(0, heapsize, heapsize-1))
-	ensures hp(a[..], heapsize) 
-	ensures multiset(a[..heapsize]) == multiset(old(a[..heapsize]))
+method {:verify true} HeapInsert1b(a: array<int>, heapsize: nat, x: int, ghost oldA: multiset<int>)
+    requires 0 < heapsize <= a.Length
+    requires multiset(a[..heapsize]) == oldA
+    requires phAndHi(a[..heapsize], IndexSet(0, heapsize, heapsize-1), heapsize-1)
+    ensures hp(a[..], heapsize)
+	ensures multiset(a[..heapsize]) == oldA
 	modifies a
 {
 	var current, parentIndex := InitCurrAndP(a,heapsize, x);
-	Heapify(a, heapsize, x, current, parentIndex);
+	Heapify(a, heapsize, x, current, parentIndex, oldA);
 }
 
 method {:verify true} InitCurrAndP(a: array<int>, heapsize: nat, x: int) returns(current: nat, parentIndex: int)
-	requires 0 < heapsize <= a.Length && a[heapsize-1] == x
-	requires multiset(a[..heapsize]) == multiset(a[..heapsize-1]+[x])
-	requires hp(a[..], heapsize-1)
-	ensures 0 <= current < a.Length && current == heapsize - 1 && parentIndex == (current - 1) / 2
+    requires 0 < heapsize <= a.Length
+    requires phAndHi(a[..heapsize], IndexSet(0, heapsize, heapsize-1), heapsize-1)
+    ensures current == heapsize - 1 && 0 <= current < a.Length && 
+    parentIndex == (current - 1) / 2
+
 	{
 	current := InitCurr(a, heapsize, x);
 	parentIndex := InitParent(a, heapsize, x, current);
 }
 
 method {:verify true} InitCurr(a: array<int>, heapsize: nat, x: int) returns(current: nat)
-	requires 0 < heapsize <= a.Length && a[heapsize-1] == x
-	requires multiset(a[..heapsize]) == multiset(a[..heapsize-1]+[x])
-	requires hp(a[..], heapsize-1)
-	ensures 0 <= current < a.Length && current == heapsize - 1
+    requires 0 < heapsize <= a.Length
+    requires phAndHi(a[..heapsize], IndexSet(0, heapsize, heapsize-1), heapsize-1)
+    ensures current == heapsize - 1 && 0 <= current < a.Length
 	{
 	LemmaCurr(a, heapsize, x);
 	current := heapsize - 1; 
 }
 lemma LemmaCurr (a: array<int>, heapsize: nat, x: int)
-	requires 0 < heapsize <= a.Length && a[heapsize-1] == x
-	requires multiset(a[..heapsize]) == multiset(a[..heapsize-1]+[x])
-	requires hp(a[..], heapsize-1)
+	requires 0 < heapsize <= a.Length
+    requires phAndHi(a[..heapsize], IndexSet(0, heapsize, heapsize-1), heapsize-1)
 	ensures 0 <= heapsize - 1 < a.Length && heapsize - 1 == heapsize - 1
 {}
-
 method {:verify true} InitParent(a: array<int>, heapsize: nat, x: int, current: nat) returns(parent: int)
-	requires 0 < heapsize <= a.Length && a[heapsize-1] == x
-	requires multiset(a[..heapsize]) == multiset(a[..heapsize-1]+[x])
-	requires hp(a[..], heapsize-1) && 0 <= current < a.Length
+    requires 0 < heapsize <= a.Length
+    requires phAndHi(a[..heapsize], IndexSet(0, heapsize, heapsize-1), heapsize-1)
+    requires current == heapsize - 1 && 0 <= current < a.Length 
 	ensures parent == (current - 1) / 2
 {
 	LemmaParent(a, heapsize, x, current);
 	parent := Parent(current);
 }
 lemma LemmaParent (a: array<int>, heapsize: nat, x: int, current: nat)
-	requires 0 < heapsize <= a.Length && a[heapsize-1] == x
-	requires multiset(a[..heapsize]) == multiset(a[..heapsize-1]+[x])
-	requires hp(a[..], heapsize-1) && 0 <= current < a.Length
-	ensures ParentFunc(current) == (current - 1) / 2
+    requires 0 < heapsize <= a.Length
+    requires phAndHi(a[..heapsize], IndexSet(0, heapsize, heapsize-1), heapsize-1)
+    requires current == heapsize - 1 && 0 <= current < a.Length 
+	ensures ParentFunc(current) == (current - 1) / 2    
 {}
 
-method {:verify true} Heapify(a: array<int>, heapsize: nat, x: int, current0: nat, parentIndex0: int)
-	requires 0 <= current0 < a.Length && current0 == heapsize - 1 && parentIndex0 == (current0 - 1) / 2
-	requires 0 < heapsize <= a.Length && a[heapsize-1] == x
-	requires multiset(a[..heapsize]) == multiset(a[..heapsize-1]+[x])
-	requires hp(a[..], heapsize-1) && ph(a[..heapsize], IndexSet(0, heapsize, current0))
-	ensures hp(a[..], heapsize)
-	ensures multiset(a[..heapsize]) == multiset(old(a[..heapsize]))
+method {:verify true} Heapify(a: array<int>, heapsize: nat, x: int, current0: nat, parentIndex0: int,ghost oldA: multiset<int>)
+    requires 0 < heapsize <= a.Length
+    requires multiset(a[..heapsize]) == oldA
+    requires phAndHi(a[..heapsize], IndexSet(0, heapsize, heapsize-1), current0)
+    requires current0 == heapsize - 1 && 0 <= current0 < a.Length && 
+    parentIndex0 == (current0 - 1) / 2
+    ensures hp(a[..], heapsize)
+	ensures multiset(a[..heapsize]) == oldA
 	modifies a
 {
 	var current, parentIndex := current0, parentIndex0; 
-	while (Guard1(a, current, parentIndex))
-		invariant WhileInv(a[..], heapsize, x, current, parentIndex, old(a[..heapsize]))
+	while (Guard1(a, current, parentIndex,heapsize))
+		invariant WhileInv(a, heapsize, x, current, parentIndex, multiset(old(a[..heapsize])))
 		decreases current
 	{ 
-		current, parentIndex := LoopBody(a, heapsize, x, current, parentIndex, old(a[..heapsize]));	
+		current, parentIndex := LoopBody(a, heapsize, x, current, parentIndex, multiset(old(a[..heapsize])));
 	}
 	// WhileInv && !Guard1
 }
-predicate method Guard1(a: array<int>, current: nat, parentIndex: int)
-	requires 0 <= current < a.Length && parentIndex == (current - 1) / 2
-	reads a
+
+predicate method Guard1(a: array<int>, current: nat, parentIndex: int, heapsize: nat)
+    reads a
 {
-	current > 0 && a[current] > a[parentIndex]
-}
-predicate WhileInv(a: seq<int>, heapsize: nat, x:int, current: nat,parentIndex: int, oldA: seq<int>)
-	requires 0 <= current < |a|
-	requires 0 < heapsize <= |a|
-{
-	multiset(a[..heapsize]) == multiset(oldA[..]) &&
-	ph(a[..], IndexSet(0, heapsize, current))
+	0 < current < heapsize <= a.Length && 
+    0 <= parentIndex < heapsize <= a.Length &&
+    a[current] > a[parentIndex]
 }
 
+predicate WhileInv(a: array<int>, heapsize: nat, x:int, current: nat,parentIndex: int, oldA: multiset<int>)
+    reads a
+{
+    parentIndex == (current - 1) / 2 &&
+	0 < heapsize <= a.Length && multiset(a[..heapsize]) == oldA &&
+	phAndHi(a[..heapsize], IndexSet(0, heapsize, current),current)
+}
 
-method {:verify true} LoopBody(a: array<int>, heapsize: nat, x: int, current0: nat, parentIndex0: int, oldA: seq<int>) returns (current: nat, parentIndex: int)
-	requires 0 <= current0 < a.Length && 0 < heapsize <= a.Length && 0 <= parentIndex0 < a.Length
-	requires Guard1(a,current0,parentIndex0) && WhileInv(a[..],heapsize,x,current0,parentIndex0,oldA)
-	ensures WhileInv(a[..], heapsize, x, current, parentIndex, oldA)
+method {:verify true} LoopBody(a: array<int>, heapsize: nat, x: int, current0: nat, parentIndex0: int, ghost oldA: multiset<int>) returns (current: nat, parentIndex: int)
+    requires 0 < heapsize <= a.Length
+    requires multiset(a[..heapsize]) == oldA
+    requires Guard1(a, current0, parentIndex0,heapsize) && WhileInv(a, heapsize, x, current0, parentIndex0, oldA)
+    ensures WhileInv(a, heapsize, x, current, parentIndex, oldA)
 	modifies a
 {
 	swap(a, heapsize, x, current0, parentIndex0, oldA); 
-	current, parentIndex := LoopBody1(a,heapsize,x,current0,parentIndex0);
-	// current := parentIndex; 
-	// parentIndex := Parent(current);
+	// current, parentIndex := setCAndP(a,heapsize,x,current0,parentIndex0,oldA);
 }
 
-lemma {:verify true} Lemma3(a: array<int>, heapsize: nat, x: int, current: nat, parentIndex: int, oldA: seq<int>) 
-	requires 0 <= current < a.Length && 0 < heapsize <= a.Length && 0 <= parentIndex < a.Length
-	requires Guard1(a,current,parentIndex) && WhileInv(a[..],heapsize,x,current,parentIndex,oldA)
-	ensures current > 0 && WhileInv(a[..parentIndex] + [a[parentIndex]] + a[parentIndex+1..current] + [a[current]],heapsize,x,parentIndex,current,oldA)
-{}
+method {:verify true} swap (a: array<int>, heapsize: nat, x: int, current: nat, parentIndex: int,ghost oldA: multiset<int>) 
+    requires Guard1(a, current, parentIndex,heapsize)
+    requires WhileInv(a, heapsize, x, current, parentIndex, oldA)
+    ensures var newA := a[..][current := a[parentIndex]][parentIndex := a[current]];
+    // ensures var newA := a[..parentIndex]+[a[current]]+a[parentIndex+1..current]+[a[parentIndex]]+a[current+1..heapsize];
+    && multiset(newA[..heapsize]) == oldA &&
+    0 < heapsize <= a.Length &&
+    phAndHi(newA[..heapsize], IndexSet(0, heapsize, parentIndex),parentIndex)
+	modifies a
+{
+	Lemma2(a ,heapsize,x,current,parentIndex,oldA);
+	a[current], a[parentIndex] := a[parentIndex], a[current];
+}
+
+lemma Lemma2(a: array<int>, heapsize: nat, x: int, current: nat, parentIndex: int, oldA: multiset<int>) 
+    requires Guard1(a, current, parentIndex,heapsize)
+    requires WhileInv(a, heapsize, x, current, parentIndex, oldA)
+    ensures var newA := a[..][current := a[parentIndex]][parentIndex := a[current]];
+    && multiset(newA[..heapsize]) == oldA &&
+    0 < heapsize <= a.Length &&
+    phAndHi(newA[..heapsize], IndexSet(0, heapsize, parentIndex),parentIndex)
+{
+    var newA := a[..][current := a[parentIndex]][parentIndex := a[current]];
+    var sParent := IndexSet(0, heapsize, parentIndex);
+    var sCurr := IndexSet(0, heapsize, current);
+    var q,k:= newA[..heapsize], parentIndex;
+    var bliPAndC := IndexSet(0, heapsize, parentIndex) - {current};
+
+    assert ph(a[..heapsize], IndexSet(0, heapsize, current));
+    assert hi(a[..heapsize],IndexSet(0, heapsize, current),parentIndex);
+    assert lo(a[..heapsize],IndexSet(0, heapsize, current),parentIndex) ==>
+    lo(newA[..heapsize],IndexSet(0, parentIndex, parentIndex),current);
+    
+    assert hi(newA[..heapsize],IndexSet(0, heapsize, parentIndex),current);
+
+    // (forall j :: j in sParent && AncestorIndex(current, j) ==> newA[current] >= newA[j]) &&
+    // (forall j :: j in sParent && AncestorIndex(j, current) ==> newA[j] >= newA[current]);
 
 
-method Main() {
-	var a := new int[8];
-	a[0] := 6;
-	a[1] := 4;
-	a[2] := 5;
-	a[3] := 3;
-	a[4] := 2;
-	a[5] := 0;
-	a[6] := 1;
-	HeapInsert(a, 7, 8);
-	print a[..];
+    // assert forall j :: j in s && AncestorIndex(k, j) ==> q[k] >= q[j];
+    // assert forall i,j :: i in bliPAndC && j in bliPAndC && AncestorIndex(i, j) ==> q[i] >= q[j];
+    // assert forall i,j :: i in s && j in s && AncestorIndex(i, j) ==> q[i] >= q[j];
 }
