HeapInsertOld.dfy
@@ -1,0 +1,253 @@
+// include "CCPR191-HeapSort-complete-30Dec18.dfy"
+
+method {:verify true} Parent(index: nat) returns (p: int) 
+	ensures p == (index - 1) / 2
+	ensures p <= index
+{
+	p := (index - 1) / 2;
+}
+function {:verify true} ParentFunc(index: nat) : int 
+{
+	(index - 1) / 2
+}
+predicate AncestorIndex(i: nat, j: nat) decreases j-i 
+{ 
+	i == j || (j > 2*i && ((AncestorIndex(2*i+1, j) || AncestorIndex(2*i+2, j))))
+}
+// definition of a heap for the prefix q[..length]
+predicate hp(q: seq<int>, length: nat)
+	requires length <= |q|
+{
+	forall i,j :: 0 <= i < length && 0 <= j < length && AncestorIndex(i, j) ==> q[i] >= q[j]
+}
+// a partial heap, restricted for elements whose index is in the given set
+predicate ph(q: seq<int>, s: set<nat>, k: nat)
+	requires (forall e :: e in s ==> e < |q|)
+{
+	(forall i,j :: i in s && j in s && AncestorIndex(i, j) ==> q[i] >= q[j]) &&
+	forall j :: j in s && AncestorIndex(k, j) ==> q[k] >= q[j]
+}
+// element k is a valid heap element (in the given range) with respect to its ancestors (lower indices)
+predicate lo(q: seq<int>, l: nat, h: nat, k: nat)
+	requires l <= h <= |q| && k < |q|
+{
+	forall i :: l <= i < h && AncestorIndex(i, k) ==> q[i] >= q[k]
+}
+// element k is a valid heap element (in the given range) with respect to its descendents (higher indices)
+predicate hi(q: seq<int>, l: nat, h: nat, k: nat)
+	requires l <= h <= |q| && k < |q|
+{
+	forall j :: l <= j < h && AncestorIndex(k, j) ==> q[k] >= q[j]
+}
+// the suffix q[i..] holds elements in their final (sorted) positions
+//fn
+function IndexSet(start: nat, end: nat, except: nat): set<nat> {
+	 set i: nat | start <= i < end && i != except }
+
+method {:verify true} HeapInsert(a: array<int>, heapsize: nat, x: int)
+	requires 0 <= heapsize < a.Length
+	requires hp(a[..], heapsize)
+	ensures hp(a[..], heapsize+1)
+	ensures multiset(a[..heapsize+1]) == multiset(old(a[..heapsize])+[x])
+	modifies a
+{
+	// BottomInsertLemma(a ,heapsize, x);
+	var newHeapsize := BottomInsert(a, heapsize, x); //add x to a end
+	HeapInsert1(a, newHeapsize, x, old(a[..]));	
+}
+method {:verify true} BottomInsert(a: array<int>, heapsize0: nat, x: int) returns (heapsize: nat)
+	requires 0 <= heapsize0 < a.Length
+	requires hp(a[..], heapsize0)
+	ensures heapsize0 == heapsize-1 && 0 < heapsize <= a.Length
+	ensures multiset(a[..heapsize]) == multiset(old(a[..heapsize - 1]+[x]))
+	ensures a[heapsize-1] == x && 0 < heapsize <= a.Length
+	ensures ph(a[..heapsize], IndexSet(0, heapsize, heapsize-1))
+	modifies a
+{
+	Lemma1(a[..heapsize0]+[x]+a[heapsize0+1..] , heapsize0+1, x, a);
+	a[heapsize0] := x;
+	heapsize := heapsize0 + 1;
+}
+
+lemma Lemma1 (a: seq<int>, heapsize: nat, x: int,oldA: array<int>)
+	requires 0 <= heapsize - 1 < |a| == oldA.Length
+	requires hp(a[..], heapsize - 1) && a[..] == oldA[..heapsize-1]+[x]+oldA[heapsize..]
+	ensures heapsize == heapsize && heapsize <= |a|
+	ensures multiset(a[..heapsize]) == multiset(oldA[..heapsize-1]+[x])
+	ensures a[heapsize-1] == x && 0 < heapsize <= |a|
+	ensures ph(a[..heapsize], IndexSet(0, heapsize, heapsize-1))
+{	
+}
+
+method {:verify true} HeapInsert1(a: array<int>, heapsize: nat, x: int, ghost oldA: seq<int>)
+	requires 0 < heapsize <= a.Length == |oldA| && a[heapsize-1] == x
+	requires multiset(a[..heapsize]) == multiset(oldA[..heapsize-1]+[x])
+	requires hp(a[..], heapsize-1) && ph(a[..heapsize], IndexSet(0, heapsize, heapsize-1))
+	ensures hp(a[..], heapsize) 
+	ensures multiset(a[..heapsize]) == multiset(oldA[..heapsize-1]+[x])
+	modifies a
+{
+	var current, parentIndex := InitCurrAndP(a,heapsize, x, oldA);
+	Heapify(a, heapsize, x, current, parentIndex, oldA);
+}
+
+method {:verify true} InitCurrAndP(a: array<int>, heapsize: nat, x: int, ghost oldA: seq<int>) returns(current: nat, parentIndex: int)
+	requires 0 < heapsize <= a.Length == |oldA| && a[heapsize-1] == x
+	requires multiset(a[..heapsize]) == multiset(oldA[..heapsize-1]+[x])
+	requires hp(a[..], heapsize-1) && ph(a[..heapsize], IndexSet(0, heapsize, heapsize-1))
+	ensures current == heapsize - 1 && 0 <= current < a.Length && parentIndex == (current - 1) / 2
+	{
+	current := InitCurr(a, heapsize, x);
+	parentIndex := InitParent(a, heapsize, x, current);
+}
+
+method {:verify true} InitCurr(a: array<int>, heapsize: nat, x: int) returns(current: nat)
+	requires 0 < heapsize <= a.Length && a[heapsize-1] == x
+	requires multiset(a[..heapsize]) == multiset(a[..heapsize-1]+[x])
+	requires hp(a[..], heapsize-1)
+	ensures 0 <= current < a.Length && current == heapsize - 1
+	{
+	LemmaCurr(a, heapsize, x);
+	current := heapsize - 1; 
+}
+lemma LemmaCurr (a: array<int>, heapsize: nat, x: int)
+	requires 0 < heapsize <= a.Length && a[heapsize-1] == x
+	requires multiset(a[..heapsize]) == multiset(a[..heapsize-1]+[x])
+	requires hp(a[..], heapsize-1)
+	ensures 0 <= heapsize - 1 < a.Length && heapsize - 1 == heapsize - 1
+{}
+
+method {:verify true} InitParent(a: array<int>, heapsize: nat, x: int, current: nat) returns(parent: int)
+	requires 0 < heapsize <= a.Length && a[heapsize-1] == x
+	requires multiset(a[..heapsize]) == multiset(a[..heapsize-1]+[x])
+	requires hp(a[..], heapsize-1) && 0 <= current < a.Length && current == heapsize - 1
+	ensures parent == (current - 1) / 2
+{
+	LemmaParent(a, heapsize, x, current);
+	parent := Parent(current);
+}
+lemma LemmaParent (a: array<int>, heapsize: nat, x: int, current: nat)
+	requires 0 < heapsize <= a.Length && a[heapsize-1] == x
+	requires multiset(a[..heapsize]) == multiset(a[..heapsize-1]+[x])
+	requires hp(a[..], heapsize-1) && 0 <= current < a.Length
+	ensures ParentFunc(current) == (current - 1) / 2
+{}
+
+method {:verify true} Heapify(a: array<int>, heapsize: nat, x: int, current0: nat, parentIndex0: int,ghost oldA: seq<int>)
+	requires current0 == heapsize - 1 && parentIndex0 == (current0 - 1) / 2
+	requires 0 <= current0 <= heapsize -1 < a.Length
+	requires a.Length == |oldA|
+	requires 0 < heapsize <= a.Length && a[heapsize-1] == x
+	requires multiset(a[..heapsize]) == multiset(oldA[..heapsize-1]+[x])
+	requires hp(a[..], heapsize-1) && ph(a[..heapsize], IndexSet(0, heapsize, current0))
+	ensures hp(a[..], heapsize)
+	ensures multiset(a[..heapsize]) == multiset(old(a[..]))
+	modifies a
+{
+	var current, parentIndex := current0, parentIndex0; 
+	// assert current0 > 0;
+	// assert a[current] > a[parentIndex];
+	while (Guard1(a[..], current, parentIndex))
+		invariant WhileInv(a[..], heapsize, x, current, parentIndex, old(a[..]))
+		decreases current
+	{ 
+		current, parentIndex := LoopBody(a, heapsize, x, current, parentIndex, old(a[..]));
+	}
+	// WhileInv && !Guard1
+}
+predicate method Guard1(a: seq<int>, current: nat, parentIndex: int)
+	requires 0 <= parentIndex <= current < |a| && parentIndex == (current - 1) / 2
+{
+	current > 0 && a[current] > a[parentIndex]
+}
+predicate WhileInv(a: seq<int>, heapsize: nat, x:int, current: nat,parentIndex: int, oldA: seq<int>)
+	requires 0 < heapsize <= |a|
+	requires 0 <= current < |a|
+	requires |a| == |oldA|
+{
+	multiset(a[..heapsize]) == multiset(oldA[..heapsize]) &&
+	ph(a[..], IndexSet(0, heapsize, current))
+}
+
+
+method {:verify true} LoopBody(a: array<int>, heapsize: nat, x: int, current0: nat, parentIndex0: int, ghost oldA: seq<int>) returns (current: nat, parentIndex: int)
+	requires  0 <= parentIndex0 <= current0 <= heapsize-1 < a.Length == |oldA| && 0 < heapsize <= a.Length
+	requires parentIndex0 == (current0 - 1) / 2 && Guard1(a[..],current0,parentIndex0)
+	requires WhileInv(a[..],heapsize,x,current0,parentIndex0,oldA[..])
+	ensures WhileInv(a[..], heapsize, x, current, parentIndex, oldA[..])
+	modifies a
+{
+	swap(a, heapsize, x, current0, parentIndex0, oldA); 
+	current, parentIndex := setCAndP(a,heapsize,x,current0,parentIndex0,oldA);
+}
+method {:verify true} swap (a: array<int>, heapsize: nat, x: int, current: nat, parentIndex: int,ghost oldA: seq<int>) 
+	requires 0 <= parentIndex <= current <= heapsize-1 < a.Length == |oldA| && 0 < heapsize <= a.Length
+	requires parentIndex == (current - 1) / 2 && Guard1(a[..],current,parentIndex)
+	requires WhileInv(a[..],heapsize,x,current,parentIndex,oldA)
+	ensures current > 0 && multiset(a[..heapsize]) == multiset(old(a[..heapsize]))
+	ensures	ph(a[..], IndexSet(0, heapsize, parentIndex))
+	modifies a
+{
+	// Lemma3(a[..],heapsize,x,current,parentIndex,oldA);
+	a[current], a[parentIndex] := a[parentIndex], a[current];
+}
+
+// lemma {:verify true} Lemma3(a: seq<int>, heapsize: nat, x: int, current: nat, parentIndex: int, oldA: seq<int>)
+// 	requires parentIndex == (current - 1) / 2 && current > 0 && |a| == |oldA|
+// 	requires 0 < heapsize <= |a[..]| && multiset(a[..heapsize]) == multiset(oldA[..heapsize])
+// 	requires 0 <= parentIndex <= current <= heapsize-1 < |a[..]| == |oldA| 
+// 	ensures current > 0 && ph(a[..], IndexSet(0, heapsize, parentIndex))
+// 	ensures multiset(a[..parentIndex]+[a[current]]+a[parentIndex+1..current]+[a[parentIndex]]+a[current+1..heapsize]) == multiset(oldA[..heapsize])
+// {
+// 	// var newA := a[..parentIndex]+[a[current]]+a[parentIndex+1..current]+[a[parentIndex]]+a[current+1..heapsize];
+// 	// var originA := a[..parentIndex]+[a[parentIndex]]+a[parentIndex+1..current]+[a[current]]+a[current+1..heapsize];
+// 	// assert 0 < heapsize <= |originA|;
+// 	// assert 0 < heapsize <= |newA|;
+// 	// assert 0 <= current < |newA|;
+// 	// assert |originA| == heapsize == |newA| == |a[..heapsize]|;
+// 	// assert multiset(newA[..parentIndex]+newA[parentIndex+1..current]+newA[current+1..heapsize]) == multiset(a[..parentIndex]+a[parentIndex+1..current]+a[current+1..heapsize]);
+//  	// assert multiset(newA[..heapsize]) == multiset(a[..heapsize]);
+// 	// assert multiset(a[..parentIndex]+[a[current]]+a[parentIndex+1..current]+[a[parentIndex]]+a[current+1..heapsize]) == multiset(oldA[..heapsize]);
+// }
+
+method setCAndP(a: array<int>, heapsize: nat, x: int, current0: nat, parentIndex0: int, ghost oldA: seq<int>) returns(current: nat, parentIndex: int)
+	requires  0 <= parentIndex0 <= current0 <= heapsize-1 < a.Length == |oldA| && 0 < heapsize <= a.Length
+	requires current0 > 0 && parentIndex0 == (current0 - 1) / 2
+	requires multiset(a[..heapsize]) == multiset(oldA[..heapsize])
+	ensures current < current0 && parentIndex <= parentIndex0
+	ensures WhileInv(a[..], heapsize, x, current, parentIndex, oldA)
+
+{
+	Lemma4(a,heapsize,x,current0,parentIndex0,oldA);
+	current := parentIndex0; 
+	parentIndex := Parent(current);
+}
+
+lemma {:verify true} Lemma4(a: array<int>, heapsize: nat, x: int, current: nat, parentIndex: int, oldA: seq<int>)
+	requires  0 <= parentIndex <= current <= heapsize-1 < a.Length == |oldA| && 0 < heapsize <= a.Length
+	requires current > 0 && parentIndex == (current - 1) / 2
+	requires multiset(a[..heapsize]) == multiset(oldA[..heapsize])
+	ensures parentIndex < current && ParentFunc(current) <= parentIndex
+	ensures WhileInv(a[..], heapsize, x, parentIndex, ParentFunc(current), oldA)
+{
+	assert 0 < heapsize <= a.Length;
+	assert 0 <= current < a.Length;
+	assert a.Length == |oldA|;
+
+	assert multiset(a[..heapsize]) == multiset(oldA[..heapsize]);
+	assert ph(a[..], IndexSet(0, heapsize, current));
+}
+
+
+method Main() {
+	var a := new int[8];
+	a[0] := 6;
+	a[1] := 4;
+	a[2] := 5;
+	a[3] := 3;
+	a[4] := 2;
+	a[5] := 0;
+	a[6] := 1;
+	HeapInsert(a, 7, 8);
+	print a[..];
+}
